main.ml
@@ -1,27 +1,34 @@
-open Lazykoq.Lazykoq ;;
+open Lazykoq;;
 
-(*
-let result = Parser.program Lexer.token (Lexing.from_channel stdin) ;;
-*)
+let rec range n m = if n == m then [n] else n::(range (n+1) m);;
 
-(*
-let _ =
-  try
-    let lexbuf = Lexing.from_channel stdin in
-      let rec loop () =
-        let result = Parser.program Lexer.token lexbuf in
-          print_endline (List.fold_left (fun ans ch -> (Char.escaped ch) ^ ans) "" (string_of_expr result)); print_endline "done."; flush stdout; loop ()
-        in
-        loop ()
-     with End_of_file -> flush stdout; exit 0
+let charList_of_string str = List.map (fun n -> str.[n]) (range 0 ((String.length str) - 1));;
 
-*)
+(* argv.(0) はプログラム名 *)
+let lazySrc = if (Array.length Sys.argv) > 1 then Sys.argv.(1) else "./sample/echo.lazy" ;;
 
+let srcChannel = open_in lazySrc ;;
 
-let fileName = if (Array.length Sys.argv) > 1 then Sys.argv.(1) else "./sample/echo.lazy" ;;
-let channel = open_in fileName ;;
+let srcLambda =
+  try 
+    let lexbuf = Lexing.from_channel srcChannel in
+      Parser.program Lexer.token lexbuf
+  with Parsing.Parse_error -> Lz.i ;;
 
-print_endline (input_line channel) ;;
-print_int (Array.length Sys.argv) ;;
+let string_of_charList chLst = (List.fold_left (fun ans ch -> (Char.escaped ch) ^ ans) "" (List.rev chLst))
 
-close_in channel ;;
+let string_of_expr lmd =
+  let chLst = (Lz.charList_of_expr lmd) in
+    string_of_charList chLst ;;
+
+let input_expr = 
+  let input_string = input_line stdin in
+    Lz.expr_of_string (charList_of_string input_string) ;;
+
+let result_string = 
+  let result_expr = (Lz.getOpt (Lz.eval (Lz.A (srcLambda, input_expr))) (Lz.i)) in
+    (Lz.string_of_churchStream result_expr);;
+
+print_endline (string_of_charList result_string) ;;
+
+close_in srcChannel ;;
